finally finished day 5. still have some sorries, but I need to move on

Utils.lean
@@ -17,35 +17,75 @@ def windows (n : Nat) (l : List α) : List (List α) :=
     |> List.map (λ (i, x) => (i / n, x)) 
     |> List.groupBy (λ (i, _) (j, _) => i = j)
     |> List.map (List.map Prod.snd)
-    
-def enum {α} (l : List α) : List (Fin l.length × α) :=
-  help l (Fin.mk 0 _)
-  -- match l with
-  -- | [] => []
-  -- | h :: tl => (Fin.mk tl.length (by simp_arith), h) :: (enum tl).map (λ (f, a) => (Fin.succ f, a))
-where help {α} (l : List α) (acc : Fin l.length) : List (Fin l.length × α) :=
+
+def finCastUp {n : Nat} (f : Fin n) (m : Nat) (lt : n <= m) : Fin m :=
+  Fin.mk 
+    (f.val)
+    (by simp_arith exact Nat.le_trans f.isLt lt)
+
+def enumFinAx {α : Type u} (l : List α) : List (Fin l.length × α) :=
   match l with
   | [] => []
-  | hd :: tl => (acc, hd) :: help l (acc.add (Fin.mk 1 _))
+  | hd :: tl => let tl' := enumFinAx tl
+                let n := (hd :: tl).length
+                let f : Fin n := Fin.ofNat tl'.length
+                let fix : List (Fin n × α) :=
+                  (List.map
+                    (λ (x : Fin tl.length × α) =>
+                      let p : tl.length <= n := by simp_arith
+                      (finCastUp x.fst n p, x.snd))
+                    tl')
+                (f, hd) :: fix
+                
+def enumFin {α : Type u} (l : List α) : List (Fin l.length × α) :=
+  -- l |> List.reverse |> enumFinAx |> List.reverse
+  let l' := l.reverse |> enumFinAx
+    
+  -- cast the list to the right type
+  let l'' : List (Fin l.length × α) := by
+    have eq : l.length = l.reverse.length := by induction l <;> simp
+    rw [eq]
+    exact l'
+      
+  -- reverse the list again to get the right order
+  l'' |> List.reverse
   
 def List.mkLength {α} (default : α) (n : Nat) : List α :=
   match n with
   | 0 => []
   | n+1 => default :: (mkLength default n)
   
-theorem List.mkLengthCorrect {α} {default : α} {n : Nat} : (List.mkLength default n).length = n := by
+theorem List.mkLengthCorrect {α} {default : α} {n : Nat}
+        : (List.mkLength default n).length = n := by
   induction n with
   | zero => simp [mkLength]
   | succ n IH => simp [mkLength] exact IH
   
-theorem enum_preserves_length {α : Type} (l : List α) : l.length = (Utils.enum l).length := by
+-- example (α : Type u) (hd : α) (tl : List α)
+--   : enumFin (hd :: tl) = (0, hd) :: enumFin tl := by simp
+  
+-- theorem enumFin_keeps_elems {α : Type u} (l : List α)
+--         : List.map Prod.snd (enumFin l) = l := by
+--   induction l with
+--   | nil => simp [List.map]
+--   | cons hd tl IH =>
+--          simp [enumFin]
+--          match (Eq.symm IH) with
+--          | Eq.refl tl =>
+--            rw [<- IH]
+--            simp [List.reverse, enumFin, enumFinAx, List.reverseAux, List.map, *]
+           
+
+-- theorem enumFin_succ {α : Type u} (hd : α) (tl : List α)
+--         : (enumFin (hd :: tl)).length = 1 + (enumFin tl).length := by
+--   simp [enumFin]
+--   rw [List.reverse_cons]
+  
+theorem enumFin_preserves_length {α : Type u} (l : List α) : l.length = (enumFin l).length := by
   induction l with
-  | nil => simp [enum]
-  | cons hd tl H => simp [enum] exact H
-
--- match enum tl with
--- | [] => [(Fin.mk 0 _, h)]
--- | (f, e) :: rst => (Fin.mk (f + 1) _, h) :: (Fin.mk f _, e) :: rst
-                
-
+  | nil => simp [enumFin, List.length]
+  | cons hd tl H =>
+    simp
+    sorry
+    
 end Utils
