Bug.lean
@@ -1,0 +1,17 @@
+abbrev Vector (α : Type u) (n : Nat) := { l : List α // l.length = n }
+
+def Vector.enum {α : Type u} {n : Nat} (l : Vector α n) : Vector (Fin n × α) n :=
+  match Nat.decLt 0 n with
+  | isTrue p =>
+    let l' := l.val.map (λ a => (Fin.mk 0 p, a))
+    let p' : List.length l' = n := by
+      induction l.property with
+      | refl => simp
+    ⟨ l', p' ⟩
+  | isFalse _ =>
+    let p := by
+      have lprop := l.property
+      simp_arith [*] at *
+      subst n
+      rfl
+    ⟨ [], p ⟩
