Dec5.lean
@@ -19,21 +19,28 @@ def Vector.fromList {α} (l : List α) : Vector α l.length := ⟨ l,  rfl ⟩
 
 def Vector.mkSize {α} (default : α) (n : Nat) : Vector α n :=
   ⟨ Utils.List.mkLength default n, Utils.List.mkLengthCorrect ⟩
-    
+  
+-- def typeq_preserves_list_len {α β} (H : Eq α β) (l : List α) : l.length = (H ▸ l).length := by
+--   induction H with
+--   | refl => rfl
 
 -- TODO! fix this definition. how the heck does type equality work?
-def Vector.enum {α} {n} (l : Vector α n) : Vector (Fin n × α) n :=
+def Vector.enum {α : Type u} {n : Nat} (l : Vector α n) : Vector (Fin n × α) n :=
   -- this is a proof that List (Fin l.length × α) = List (Fin n × a)
-  let l' : List (Fin n × α) := (Eq.symm l.property) ▸ Utils.enum l.val
+  let l' : List (Fin n × α) := (Eq.symm l.property) ▸ Utils.enumFin l.val
+  
+  -- why does this proof not work?
   let p : List.length l' = n := by
-    have leq : l.val.length = l'.length := sorry
-    rw [<- leq]
-    exact l.property
+    have lprop := l.property
+    sorry
+    -- induction lprop
+    -- simp
+    -- have x := Utils.enumFin_preserves_length l.val
+    -- exact Eq.symm x
+    -- exact Eq.symm (Utils.enumFin_preserves_length l.val)
 
   ⟨ l', p ⟩
-  
-#eval Vector.enum (Vector.fromList ['a', 'b', 'c'])
-
+ 
 notation a ":::" b => Vector.cons a b
 
 structure StackMachine (n : Nat) where
@@ -46,18 +53,35 @@ def StackMachine.empty : StackMachine 0 :=
 def StackMachine.addCol {n : Nat} (sm : StackMachine n) : StackMachine (n + 1) :=
   StackMachine.mk $ sm.stacks.cons []
   
+def StackMachine.endIdx {n : Nat} (sm : StackMachine n) (H : n > 0) : Fin n :=
+  let len := sm.stacks.length - 1
+  Fin.mk len (by simp_arith [Vector.length, Nat.sub]
+                 cases n with
+                 | zero => contradiction
+                 | succ n' => simp)
+                 
+def StackMachine.takeN {n : Nat} (frm : Fin n) (c : Nat) (sm : StackMachine n) : (List Char × StackMachine n) :=
+  let stack := (sm.stacks.nth frm).enum
+  let ltPred : (Nat × Char) -> Bool := λ x => x.fst < c
+  let elems := stack.takeWhile ltPred |> List.map Prod.snd
+  let drop := stack.dropWhile ltPred |> List.map Prod.snd
+  (elems, StackMachine.mk $ sm.stacks.set frm drop)
+  
 def StackMachine.take {n : Nat} (frm : Fin n) (sm : StackMachine n) : Option (Char × StackMachine n) :=
-  let stack := sm.stacks.nth frm
-  match stack with
-  | h :: tl => (h, StackMachine.mk $ sm.stacks.set frm tl)
-  | [] => none
+  match sm.takeN frm 1 with
+  | ([c], sm') => some (c, sm')
+  | _ => none
+  
+def StackMachine.placeN {n : Nat} (to : Fin n) (cs : List Char) (sm : StackMachine n) : StackMachine n :=
+  let stack := sm.stacks.nth to
+  StackMachine.mk $ sm.stacks.set to (cs ++ stack)
   
 def StackMachine.place {n : Nat} (to : Fin n) (c : Char) (sm : StackMachine n) : StackMachine n :=
-  let stack := sm.stacks.nth to
-  StackMachine.mk $ sm.stacks.set to (c :: stack)
+  sm.placeN to [c]
   
 -- Move `num` boxes from stack `frm` to stack `to`
-def StackMachine.move {n : Nat} (num : Nat) (frm : Fin n) (to : Fin n) (sm : StackMachine n) : StackMachine n :=
+def StackMachine.move {n : Nat} (num : Nat) (frm : Fin n) (to : Fin n) (sm : StackMachine n)
+    : StackMachine n :=
   match num with
   | 0 => sm
   | n + 1 => 
@@ -66,11 +90,28 @@ def StackMachine.move {n : Nat} (num : Nat) (frm : Fin n) (to : Fin n) (sm : Sta
                | none => sm
     sm'.move n frm to
     
+def StackMachine.move9001 {n : Nat} (num : Nat) (frm : Fin n) (to : Fin n) (sm : StackMachine n)
+    : StackMachine n :=
+  let (chars, sm') := sm.takeN frm num
+  sm'.placeN to chars
+    
+def StackMachine.top {n : Nat} (sm : StackMachine n) : List Char :=
+  match Nat.decLt 0 n with
+  | isTrue p => h sm (sm.endIdx p)
+  | isFalse _ => []
+where h {n : Nat} (sm : StackMachine n) (acc : Fin n) : List Char :=
+  match acc with
+  | ⟨0, _⟩ =>
+    match sm.take acc with
+    | some (el, _) => [el]
+    | none => []
+  | ⟨i+1, lt⟩ =>
+    let f := ⟨i, Nat.lt_of_succ_lt lt⟩
+    match sm.take acc with
+    | some (el, _) => el :: h sm f
+    | none => h sm f
+    
 def data : String := "data/dec5.txt"
-
--- def List.foldl_dep {β} {α : (x : β) -> γ} (f : α → β → α) : (init : α) → List β → α
---   | a, List.nil      => a
---   | a, List.cons b l => foldl_dep f (f a b) l
 
 def parseStartingMachine (l : List String) : Option ((n : Nat) × StackMachine n) := do
   -- clean up the input
@@ -95,27 +136,58 @@ def parseStartingMachine (l : List String) : Option ((n : Nat) × StackMachine n
     cleanVecs.foldl
       (λ acc v =>
         let v' := v.enum
-        v'.val.foldl (λ acc (p, c) => acc.place p c) acc)
+        v'.val.foldl (λ acc (p, c) => if c ≠ ' ' then acc.place p c else acc) acc)
       sm
                  
   pure ⟨ hd.length, sm' ⟩
-
-#eval do (<- Utils.lines data)
-      |> List.groupBy (λ (x y : String) =>
-           (x.startsWith "move" && y.startsWith "move") || (!x.startsWith "move" && !y.startsWith "move"))
-      |> (List.get! · 0)
-      |> parseStartingMachine
-      |> pure
+  
+def parseMoves (n : Nat) (input : String) : Option (Nat × Fin n × Fin n) := do
+  let s := input.split (· = ' ')
+  let countStr <- s.get? 1
+  let frmStr <- s.get? 3
+  let toStr <- s.get? 5
+  
+  let count <- String.toNat? countStr
+  let frm <- String.toNat? frmStr
+  let frm' := frm - 1
+  let to <- String.toNat? toStr
+  let to' := to - 1
+  
+  match frm'.decLt n, to'.decLt n with
+  | isTrue fp, isTrue tp => return (count, Fin.mk frm' fp, Fin.mk to' tp)
+  | _, _ => none
 
 def run : IO Unit := do
+  let lines <- Utils.lines data
+  let split := lines.groupBy (λ (x y : String) =>
+           (x.startsWith "move" && y.startsWith "move")
+            || (!x.startsWith "move" && !y.startsWith "move"))
+            
+  let initMachineInput := split.get! 0
+  let movesInput := split.get! 1
 
-  let part1 := ()
-  let part2 := ()
+  let part1 := do
+    let ⟨n, start⟩ <- parseStartingMachine initMachineInput
+    let moves := movesInput.reverse.filterMap (parseMoves n)
+    
+    let sm' : StackMachine n := moves.foldl
+           (λ acc (c, f, t) => acc.move c f t)
+           start
+    return sm'.top.reverse.asString
+
+  let part2 := do
+    let ⟨n, start⟩ <- parseStartingMachine initMachineInput
+    let moves := movesInput.reverse.filterMap (parseMoves n)
+
+    let sm' : StackMachine n := moves.foldl
+           (λ acc (c, f, t) => acc.move9001 c f t)
+           start
+    return sm'.top.reverse.asString
   
   let stdout <- IO.getStdout
   stdout.putStrLn s!"Part1: {part1}"
   stdout.putStrLn s!"Part2: {part2}"
-
-  pure ()
+  
+#eval run
 
 end Dec5
